main/ts/terse/lean/TS.lean
@@ -5,6 +5,5 @@ import TS.Types
 import TS.Stlc
 import TS.StlcProp
 import TS.MoreStlc
-import TS.Sub
 
--- Built on 2026-09-10 16:24 UTC
+-- Built on 2026-09-07 17:56 UTC
